Remov MLS.Crypto.Derived interface, slight refactor

fstar/MLS.Crypto.Derived.fst
@@ -1,8 +1,15 @@
 module MLS.Crypto.Derived
 
+open MLS.Crypto.Builtins
+open MLS.NetworkTypes
+open Comparse
+open MLS.Result
+
+
 #set-options "--fuel 0 --ifuel 0"
 
 #push-options "--ifuel 1"
+val available_ciphersuite_from_network: cipher_suite_nt -> result available_ciphersuite
 let available_ciphersuite_from_network cs =
   match cs with
   | CS_mls_128_dhkemx25519_aes128gcm_sha256_ed25519 () -> return AC_mls_128_dhkemx25519_aes128gcm_sha256_ed25519
@@ -15,6 +22,7 @@ let available_ciphersuite_from_network cs =
 #pop-options
 
 #push-options "--ifuel 1"
+val available_ciphersuite_to_network: available_ciphersuite -> cipher_suite_nt
 let available_ciphersuite_to_network cs =
   match cs with
   | AC_mls_128_dhkemx25519_aes128gcm_sha256_ed25519 -> CS_mls_128_dhkemx25519_aes128gcm_sha256_ed25519 ()
@@ -40,25 +48,42 @@ type sign_content_nt (bytes:Type0) {|bytes_like bytes|} = {
 
 %splice [ps_sign_content_nt] (gen_parser (`sign_content_nt))
 %splice [ps_sign_content_nt_length] (gen_length_lemma (`sign_content_nt))
+%splice [ps_sign_content_nt_is_valid] (gen_is_valid_lemma (`sign_content_nt))
+
+instance parseable_serializeable_sign_content_nt (bytes:Type0) {|bytes_like bytes|}: parseable_serializeable bytes (sign_content_nt bytes) = mk_parseable_serializeable ps_sign_content_nt
+
+let valid_label = s:string{b2t (normalize_term (string_is_ascii s)) /\ normalize_term (String.length s) < normalize_term ((pow2 30) - 8)}
+
+val get_mls_label: #bytes:Type0 -> {|crypto_bytes bytes|} -> label:valid_label -> Pure (mls_bytes bytes)
+  (requires True)
+  (ensures fun res -> length #bytes res == 8 + String.strlen label)
+let get_mls_label #bytes #cb label =
+  normalize_term_spec (String.strlen label);
+  normalize_term_spec ((pow2 30) - 8);
+  assert_norm (String.strlen "MLS 1.0 " == 8);
+  let bytes_mls = string_to_bytes #bytes "MLS 1.0 " in
+  let bytes_label = string_to_bytes #bytes label in
+  concat_length #bytes bytes_mls bytes_label;
+  concat #bytes bytes_mls bytes_label
+
+let sign_with_label_pre (#bytes:Type0) {|crypto_bytes bytes|} (label:valid_label) (length_content:mls_nat): bool =
+  8 + (8 + String.strlen label) + length_content < sign_max_input_length #bytes
 
 val get_sign_content: #bytes:Type0 -> {|crypto_bytes bytes|} -> label:valid_label -> content:mls_bytes bytes -> Pure bytes
   (requires sign_with_label_pre #bytes label (length #bytes content))
   (ensures fun res -> length #bytes res < sign_max_input_length #bytes)
 let get_sign_content #bytes #cb label content =
-  normalize_term_spec (String.strlen label);
-  normalize_term_spec ((pow2 30) - 8);
-  assert_norm (String.strlen "MLS 1.0 " == 8);
-  let label = string_to_bytes #bytes label in
-  concat_length #bytes (string_to_bytes #bytes "MLS 1.0 ") label;
   ((ps_to_pse ps_sign_content_nt).serialize_exact ({
-    label = concat #bytes (string_to_bytes #bytes "MLS 1.0 ") label;
+    label = get_mls_label #bytes label;
     content = content;
   }))
 
+val sign_with_label: #bytes:Type0 -> {|crypto_bytes bytes|} -> signature_key:sign_private_key bytes -> label:valid_label -> content:mls_bytes bytes{sign_with_label_pre #bytes label (length #bytes content)} -> entropy:sign_nonce bytes -> sign_signature bytes
 let sign_with_label #bytes #cb signature_key label content entropy =
   let sign_content = get_sign_content label content in
   sign_sign signature_key sign_content entropy
 
+val verify_with_label: #bytes:Type0 -> {|crypto_bytes bytes|} -> verification_key:sign_public_key bytes -> label:valid_label -> content:mls_bytes bytes{sign_with_label_pre #bytes label (length #bytes content)} -> signature:sign_signature bytes -> bool
 let verify_with_label #bytes #cb verification_key label content signature =
   let sign_content = get_sign_content label content in
   sign_verify verification_key sign_content signature
@@ -71,6 +96,7 @@ type kdf_label_nt (bytes:Type0) {|bytes_like bytes|} = {
 
 %splice [ps_kdf_label_nt] (gen_parser (`kdf_label_nt))
 
+val expand_with_label: #bytes:Type0 -> {|crypto_bytes bytes|} -> secret:bytes -> label:bytes -> context:bytes -> len:nat -> result (lbytes bytes len)
 let expand_with_label #bytes #cb secret label context len =
   assert_norm (String.strlen "MLS 1.0 " == 8);
   if not (len < pow2 16) then
@@ -89,6 +115,7 @@ let expand_with_label #bytes #cb secret label context len =
     kdf_expand secret kdf_label len
   )
 
+val derive_secret: #bytes:Type0 -> {|crypto_bytes bytes|} -> secret:bytes -> label:bytes -> result (lbytes bytes (kdf_length #bytes))
 let derive_secret #bytes #cb secret label =
   expand_with_label secret label (empty #bytes) (kdf_length #bytes)
 
@@ -113,13 +140,16 @@ let ref_hash #bytes #cb label value =
     return (hash_hash (serialize #bytes (ref_hash_input_nt bytes) ({label; value;})))
   )
 
+val make_keypackage_ref: #bytes:Type0 -> {|crypto_bytes bytes|} -> bytes -> result (lbytes bytes (hash_length #bytes))
 let make_keypackage_ref #bytes #cb buf =
   ref_hash (string_to_bytes #bytes "MLS 1.0 KeyPackage Reference") buf
 
+val make_proposal_ref: #bytes:Type0 -> {|crypto_bytes bytes|} -> bytes -> result (lbytes bytes (hash_length #bytes))
 let make_proposal_ref #bytes #cb buf =
   ref_hash (string_to_bytes #bytes "MLS 1.0 Proposal Reference") buf
 
 #push-options "--fuel 1 --ifuel 1"
+val split_randomness: #bytes:Type0 -> {|bytes_like bytes|} -> #l1:list nat -> #l2:list nat -> randomness bytes (List.Tot.append l1 l2) -> (randomness bytes l1 & randomness bytes l2)
 let rec split_randomness #bytes #bl #l1 #l2 r =
   match l1 with
   | [] -> (mk_empty_randomness bytes, r)
@@ -129,9 +159,11 @@ let rec split_randomness #bytes #bl #l1 #l2 r =
     (mk_randomness (rh, rt1), rl2)
 #pop-options
 
+val mk_zero_vector: #bytes:Type0 -> {|bytes_like bytes|} -> n:nat -> lbytes bytes n
 let mk_zero_vector #bytes #bl n =
   FStar.Math.Lemmas.pow2_le_compat n 0;
   from_nat #bytes n 0
 
+val zero_vector: #bytes:Type0 -> {|crypto_bytes bytes|} -> bytes
 let zero_vector #bytes #cb =
   mk_zero_vector #bytes (kdf_length #bytes)
